

**1.**

Write the conditional bias of the local polynomial regression estimator for  $p - \nu$  odd

$$\text{bias}[\hat{m}_\nu(x_0) \mid \mathbb{X}] = \varepsilon_{\nu+1}^T \mathbf{S}^{-1} \mathbf{c}_p \frac{\nu!}{(p+1)!} m^{(p+1)}(x_0) h^{p+1-\nu} + o_p(h^{p+1-\nu})$$

in terms of the equivalent kernel  $K_{\nu,p}^*$  (see p. 60 Eq. (4.29) in the notes).

**Answer**

Let  $(X_1, Y_1), \dots, (X_n, Y_n)$  be an independent identically distributed sample from  $(X, Y)$ , with the typical model of the form:

$$Y_i = m(X_i) + \sigma(X_i)e_i, \quad \mathbb{E}[e_i] = 0, \quad \text{Var}(e_i) = 1$$

and  $X$  and  $e$  are independent. Also, for my own sanity, note:  $\mathbb{X} = (X_1, \dots, X_n)$ .

The order- $p$  local polynomial estimator at  $x_0$  minimizes:

$$\sum_{i=1}^n \left( Y_i - \sum_{j=0}^p \beta_j (X_i - x_0)^j \right)^2 K_h(X_i - x_0), \quad K_h(u) = \frac{1}{h} K(u/h)$$

Let  $\mathbf{X}$  be the  $n \times (p+1)$  design matrix with  $(j+1)$  column  $(X_i - x_0)^j$ .

Further, let  $W = \text{diag}\{K_h(X_i - x_0)\}$ , and define:

$$S_n = \mathbf{X}^\top \mathbf{W} \mathbf{X}, \quad \hat{\beta} = S_n^{-1} \mathbf{X}^\top \mathbf{W} \mathbf{Y}$$

The estimator of the  $\nu$ th derivative is:

$$\hat{m}_\nu(x_0) = \nu! \varepsilon_{\nu+1}^\top \hat{\beta}$$

A  $(p+1)$ -term Taylor expansion gives:

$$m(X_i) = \sum_{j=0}^p \beta_j (X_i - x_0)^j + r_i, \quad \beta_j = \frac{m^{(j)}(x_0)}{j!},$$

with remainder term  $r_i$  given by:

$$r_i = \frac{m^{(p+1)}(x_0)}{(p+1)!} (X_i - x_0)^{p+1} + o_p(h^{p+1})$$

Thus:

$$\mathbb{E}[\hat{\beta} \mid \mathbb{X}] = \beta + S_n^{-1} \mathbf{X}^\top \mathbf{W} \mathbf{r}, \quad \text{bias}[\hat{\beta} \mid \mathbb{X}] = S_n^{-1} \mathbf{X}^\top \mathbf{W} \mathbf{r}$$

Let:

$$S_{n,j} = \sum_{i=1}^n (X_i - x_0)^j K_h(X_i - x_0), \quad c_n = (S_{n,p+1}, \dots, S_{n,2p+1})^\top$$

Using the remainder term:

$$\mathbf{X}^\top \mathbf{W} \mathbf{r} = \beta_{p+1} c_n + o_p((nh^{p+1}, \dots, nh^{2p+1})^\top), \quad \beta_{p+1} = \frac{m^{(p+1)}(x_0)}{(p+1)!}$$

Define:

$$H = \text{diag}(1, h, \dots, h^p), \quad \mu_j = \int u^j K(u) du,$$

And additionally:

$$S = (\mu_{j+\ell})_{0 \leq j, \ell \leq p} \quad \text{and} \quad c_p = (\mu_{p+1}, \dots, \mu_{2p+1})^\top$$

Note: There are two different moment vectors in this derivation:  $c_n = (S_{n,p+1}, \dots, S_{n,2p+1})^\top$  and  $c_p = (\mu_{p+1}, \dots, \mu_{2p+1})^\top$ . The text does also uses both, but only explicitly defines  $c_n$ . Further,  $c_n$  denotes the sample vector of weighted empirical moments while  $c_p$  is the population moment vector appearing in the asymptotic bias formula.

Continuing on, for continuous  $f_X$  at  $x_0$ ,

$$S_n \approx n f_X(x_0) H S H, \quad c_n \approx n f_X(x_0) H c_p h^{p+1}$$

Taken together:

$$\text{bias}[\hat{\beta} \mid \mathbb{X}] = H^{-1} S^{-1} c_p \beta_{p+1} h^{p+1} + o_p(h^{p+1})$$

Projecting to the  $\nu$ th derivative:

$$\text{bias}[\hat{m}_\nu(x_0) \mid \mathbb{X}] = \nu! \varepsilon_{\nu+1}^\top H^{-1} S^{-1} c_p \beta_{p+1} h^{p+1}$$

so

$$\text{bias}[\hat{m}_\nu(x_0) \mid \mathbb{X}] = \varepsilon_{\nu+1}^\top S^{-1} c_p \frac{\nu!}{(p+1)!} m^{(p+1)}(x_0) h^{p+1-\nu} + o_p(h^{p+1-\nu})$$

For  $p - \nu$  odd, the leading term does not vanish.

Now define the equivalent kernel:

$$K_{\nu,p}^*(t) = \varepsilon_{\nu+1}^\top S^{-1} (1, t, \dots, t^p)^\top K(t)$$

As given, the equivalent kernel satisfies the moment conditions:

$$\int t^q K_{\nu,p}^*(t) dt = \delta_{\nu,q} \quad 0 \leq \nu, q \leq p$$

Also:

$$\int t^{p+1} K_{\nu,p}^{\star}(t) dt = \varepsilon_{\nu+1}^{\top} S^{-1} c_p$$

Substituting this identity into the bias expression gives:

$$\text{bias}[\hat{m}_{\nu}(x_0) \mid \mathbb{X}] = \left( \int t^{p+1} K_{\nu,p}^{\star}(t) dt \right) \frac{\nu!}{(p+1)!} m^{(p+1)}(x_0) h^{p+1-\nu} + o_p(h^{p+1-\nu})$$

for  $p - \nu$  odd.

**2.**

Write the conditional variance of the local polynomial regression estimator

$$\text{Var}[\hat{m}_\nu(x_0) \mid \mathbb{X}] = \varepsilon_{\nu+1}^T \mathbf{S}^{-1} \mathbf{S}^* \mathbf{S}^{-1} \varepsilon_{\nu+1} \frac{\nu!^2 \sigma^2(x_0)}{f_X(x_0) n h^{1+2\nu}} + o_p\left(\frac{1}{n h^{1+2\nu}}\right)$$

in terms of the equivalent kernel  $K_{\nu,p}^*$  (see p. 60 Eq. (4.30) in the notes).

**Answer**

Under the same setup and assumptions of Question 1, we have:

$$\hat{m}_\nu(x_0) = \nu! \varepsilon_{\nu+1}^\top \hat{\beta}$$

Conditional on  $\mathbb{X}$ :

$$\text{Var}(Y \mid \mathbb{X}) = \text{diag}\{\sigma^2(X_i)\}$$

(which assumes independence of errors)

So:

$$\text{Var}[\hat{m}_\nu(x_0) \mid \mathbb{X}] = \nu!^2 \varepsilon_{\nu+1}^\top S_n^{-1} \mathbf{X}^\top \mathbf{W} \text{Var}(Y \mid \mathbb{X}) \mathbf{W} \mathbf{X} S_n^{-1} \varepsilon_{\nu+1}$$

Assuming  $\sigma^2(X_i) \approx \sigma^2(x_0)$  near  $x_0$  (assume  $\sigma^2(X_i)$  is smooth near  $x_0$ ),

$$\text{Var}[\hat{m}_\nu(x_0) \mid \mathbb{X}] = \nu!^2 \sigma^2(x_0) \varepsilon_{\nu+1}^\top S_n^{-1} (\mathbf{X}^\top \mathbf{W}^2 \mathbf{X}) S_n^{-1} \varepsilon_{\nu+1} [1 + o_p(1)]$$

Let:

$$H = \text{diag}(1, h, \dots, h^p), \quad \mu_j = \int u^j K(u) du, \quad \text{and } \nu_j = \mu_j^{(2)} = \int u^j K(u)^2 du$$

Note: For what follows, I use  $\nu_j$  in lieu of  $\mu_j^{(2)}$  for notational convenience.

And define:

$$\mathbf{S} = (\mu_{j+\ell})_{0 \leq j, \ell \leq p}, \quad \mathbf{S}^* = (\mu_{j+\ell}^{(2)})_{0 \leq j, \ell \leq p} = \begin{pmatrix} \nu_0 & \nu_1 & \cdots & \nu_p \\ \nu_1 & \nu_2 & \cdots & \nu_{p+1} \\ \vdots & \vdots & \ddots & \vdots \\ \nu_p & \nu_{p+1} & \cdots & \nu_{2p} \end{pmatrix} \quad (4.20)$$

With  $f_X$  continuous at  $x_0$ :

$$S_n \approx n f_X(x_0) H S H, \quad \mathbf{X}^\top \mathbf{W}^2 \mathbf{X} \approx \frac{n f_X(x_0)}{h} H \mathbf{S}^* H$$

Hence

$$S_n^{-1} \approx \frac{1}{nf_X(x_0)} H^{-1} \mathbf{S}^{-1} H^{-1}$$

Substituting,

$$\text{Var}[\hat{m}_\nu(x_0) \mid \mathbb{X}] = \nu!^2 \sigma^2(x_0) \frac{1}{nf_X(x_0)} \frac{1}{h} \varepsilon_{\nu+1}^\top [H^{-1} \mathbf{S}^{-1} \mathbf{S}^* \mathbf{S}^{-1} H^{-1}] \varepsilon_{\nu+1} [1 + o_p(1)]$$

Since  $H^{-1} \varepsilon_{\nu+1} = h^{-\nu} \varepsilon_{\nu+1}$ ,

$$\text{Var}[\hat{m}_\nu(x_0) \mid \mathbb{X}] = \varepsilon_{\nu+1}^\top \mathbf{S}^{-1} \mathbf{S}^* \mathbf{S}^{-1} \varepsilon_{\nu+1} \frac{\nu!^2 \sigma^2(x_0)}{f_X(x_0) n h^{1+2\nu}} + o_p\left(\frac{1}{nh^{1+2\nu}}\right)$$

Now define the equivalent kernel:

$$K_{\nu,p}^*(t) = \varepsilon_{\nu+1}^\top \mathbf{S}^{-1} (1, t, \dots, t^p)^\top K(t)$$

Under random design with density  $f_X$ :

$$\hat{m}_\nu(x_0) = \frac{1}{nh^{\nu+1} f_X(x_0)} \sum_{i=1}^n K_{\nu,p}^* \left( \frac{X_i - x_0}{h} \right) Y_i [1 + o_p(1)]$$

Using  $\text{Var}(Y_i \mid \mathbb{X}) \approx \sigma^2(x_0)$  and assumption of independence (specifically independence of errors conditional on  $\mathbb{X}$ ),

$$\text{Var}[\hat{m}_\nu(x_0) \mid \mathbb{X}] = \frac{\nu!^2 \sigma^2(x_0)}{nh^{1+2\nu} f_X(x_0)} \int [K_{\nu,p}^*(t)]^2 dt + o_p\left(\frac{1}{nh^{1+2\nu}}\right) \quad (\text{as in 4.30})$$

**3.**

Show that the equivalent kernel satisfies the following moment condition

$$\int u^q K_{\nu,p}^*(u) du = \delta_{\nu,q} \quad 0 \leq \nu, q \leq p,$$

where  $\delta_{\nu,q} = 1$  if  $\nu = q$  and 0 else.

**Answer**

Let:

$$v_p(u) = (1, u, \dots, u^p)^\top, \quad \mathbf{S} = \int v_p(u) v_p(u)^\top K(u) du = (\mu_{j+\ell})_{0 \leq j, \ell \leq p}$$

Where we follow the typical convention:  $\mu_r = \int u^r K(u) du$ .

As defined, the equivalent kernel is of the form:

$$K_{\nu,p}^*(u) = \varepsilon_{\nu+1}^\top \mathbf{S}^{-1} v_p(u) K(u) \quad (4.27, \text{ but using } u \text{ instead of } t)$$

Where  $\varepsilon_{\nu+1}$  denotes the  $(\nu+1)$ -st canonical basis vector in  $\mathbb{R}^{p+1}$ .

For  $0 \leq q \leq p$ , the  $q$ -th moment of  $K_{\nu,p}^*$  is:

$$\int u^q K_{\nu,p}^*(u) du = \varepsilon_{\nu+1}^\top \mathbf{S}^{-1} \left( \int v_p(u) u^q K(u) du \right)$$

Define the vector

$$s_q = \int v_p(u) u^q K(u) du = \begin{pmatrix} \mu_q \\ \mu_{q+1} \\ \vdots \\ \mu_{q+p} \end{pmatrix}$$

Note:  $s_q$  is exactly the  $(q+1)$ -st column of  $\mathbf{S}$ , i.e., for  $j = 0, \dots, p$ :

$$(s_q)_{j+1} = \mu_{q+j} = \mathbf{S}_{j+1, q+1}$$

Hence  $s_q = \mathbf{S} \varepsilon_{q+1}$ .

Therefore:

$$\int u^q K_{\nu,p}^*(u) du = \varepsilon_{\nu+1}^\top \mathbf{S}^{-1} \mathbf{S} \varepsilon_{q+1} = \varepsilon_{\nu+1}^\top \varepsilon_{q+1} = \delta_{\nu,q}$$

Noting that:

$$\varepsilon_{\nu+1}^\top \varepsilon_{q+1} = \begin{cases} 1, & \nu = q, \\ 0, & \nu \neq q, \end{cases}$$

We have then proved that the equivalent kernel satisfies the moment condition

$$\int u^q K_{\nu,p}^*(u) du = \delta_{\nu,q} \quad 0 \leq \nu, q \leq p,$$

## 4.

Show that the weights  $W_\nu^n$  satisfy the following discrete moment condition

$$\sum_{i=1}^n (X_i - x_0)^q W_\nu^n \left( \frac{X_i - x_0}{h} \right) = \delta_{\nu,q} \quad 0 \leq \nu, q \leq p$$

**Answer**

Note on notation:  $\mathbf{X}$  and  $\mathbf{W}$  denote matrices, and  $W_\nu^n(\cdot)$  denotes the scalar weight function used in the local polynomial estimator (so that  $W_\nu^n((X_i - x_0)/h)$  is the weight applied to observation  $i$ ). I attempted to follow the notation of the text throughout.

That all being said, let:

$$\mathbf{X} = \begin{pmatrix} 1 & (X_1 - x_0) & \cdots & (X_1 - x_0)^p \\ \vdots & \vdots & \ddots & \vdots \\ 1 & (X_n - x_0) & \cdots & (X_n - x_0)^p \end{pmatrix}, \quad \mathbf{W} = \text{diag}(K_h(X_i - x_0))$$

And define:

$$S_n = \mathbf{X}^\top \mathbf{W} \mathbf{X}$$

Then, the order- $p$  local polynomial estimator of the  $\nu$ th derivative at  $x_0$  can be written as:

$$\hat{m}_\nu(x_0) = \sum_{i=1}^n W_\nu^n \left( \frac{X_i - x_0}{h} \right) Y_i \quad (4.25 \text{ of the text})$$

Where the weights are defined (for  $0 \leq \nu \leq p$ ) as:

$$\begin{aligned} W_\nu^n \left( \frac{X_i - x_0}{h} \right) &= \varepsilon_{\nu+1}^\top S_n^{-1} \mathbf{X}^\top \mathbf{W} e_i \\ &= \varepsilon_{\nu+1}^\top S_n^{-1} x_i K_h(X_i - x_0) \end{aligned}$$

and  $\varepsilon_{\nu+1}$  is the  $(\nu+1)$ st canonical basis vector, while  $e_i$  is the  $i$ th standard basis vector in  $\mathbb{R}^n$ .

Fix  $q \in \{0, 1, \dots, p\}$ .

The goal is to show:

$$\sum_{i=1}^n (X_i - x_0)^q W_\nu^n \left( \frac{X_i - x_0}{h} \right) = \delta_{\nu,q}$$

To that end, substituting the definition of  $W_\nu^n$  given above:

$$\begin{aligned} \sum_{i=1}^n (X_i - x_0)^q W_\nu^n \left( \frac{X_i - x_0}{h} \right) &= \sum_{i=1}^n (X_i - x_0)^q \varepsilon_{\nu+1}^\top S_n^{-1} x_i K_h(X_i - x_0) \\ &= \varepsilon_{\nu+1}^\top S_n^{-1} \left( \sum_{i=1}^n x_i (X_i - x_0)^q K_h(X_i - x_0) \right) \end{aligned}$$

Note that

$$\begin{aligned}\sum_{i=1}^n x_i (X_i - x_0)^q K_h(X_i - x_0) &= \sum_{i=1}^n x_i x_i^\top K_h(X_i - x_0) \varepsilon_{q+1} \\ &= S_n \varepsilon_{q+1}\end{aligned}$$

Where, notationally:

$$x_i = \begin{pmatrix} 1 & (X_i - x_0) & \cdots & (X_i - x_0)^p \end{pmatrix}^\top, \quad X = \begin{pmatrix} x_1^\top & \vdots & x_n^\top \end{pmatrix}$$

And where:

$$x_i^\top \varepsilon_{q+1} = (X_i - x_0)^q$$

Substituting this back into the overall equation gives:

$$\begin{aligned}\sum_{i=1}^n (X_i - x_0)^q W_\nu^n \left( \frac{X_i - x_0}{h} \right) &= \varepsilon_{\nu+1}^\top S_n^{-1} (S_n \varepsilon_{q+1}) \\ &= \varepsilon_{\nu+1}^\top \varepsilon_{q+1} \\ &= \delta_{\nu,q}\end{aligned}$$

Thus, the weights  $W_\nu^n$  satisfy the discrete moment condition:

$$\sum_{i=1}^n (X_i - x_0)^q W_\nu^n \left( \frac{X_i - x_0}{h} \right) = \delta_{\nu,q} \quad 0 \leq \nu, q \leq p$$